Add parser with correctness proof

coq/Parser.vy
@@ -1,0 +1,69 @@
+%{
+
+Require Import String.
+
+Inductive uexpr_unop : Set := | unop_neg.
+Inductive uexpr_binop : Set :=
+| binop_and
+| binop_or
+| binop_eq
+| binop_incl
+.
+
+Inductive uexpr : Set :=
+| e_string : string -> uexpr
+| e_block : list uexpr -> uexpr
+| e_list : list uexpr -> uexpr
+| e_call : string -> list uexpr -> uexpr
+| e_var : string -> uexpr
+| e_unop : uexpr_unop -> uexpr -> uexpr
+| e_binop : uexpr_binop -> uexpr -> uexpr -> uexpr
+.
+
+%}
+
+%token EOF
+%token LPAREN "(" RPAREN ")"
+%token LBRACE "{" RBRACE "}"
+%token LSQUARE "[" RSQUARE "]"
+%token COMMA "," SEMI ";"
+%token DOLLAR "$"
+%token NOT "~" AND "&" OR "|" EQ "=" IN "%"
+%token<string> STR
+
+%start<uexpr> parse_uexpr
+%type<uexpr> expr primary_expr unary_expr binary_expr
+%type<list uexpr> list(";", expr) list(",", expr)
+%type<uexpr_unop> unop
+%type<uexpr_binop> binop
+
+%%
+
+let parse_uexpr := e = expr; EOF; { e }
+
+let list(delim, x) :=
+	| { nil }
+	| h = x; { cons h nil }
+	| h = x; delim; t = list(delim, x); { cons h t }
+
+let unop := "~"; { unop_neg }
+let binop :=
+	| "&"; { binop_and }
+	| "|"; { binop_or }
+	| "="; { binop_eq }
+	| "%"; { binop_incl }
+
+let expr := binary_expr
+let primary_expr :=
+	| s = STR; <e_string>
+	| "["; l = list(",", expr); "]"; <e_list>
+	| "{"; l = list(";", expr); "}"; <e_block>
+	| s = STR; "("; l = list(",", expr); ")"; { e_call s l }
+	| "("; e = expr; ")"; { e }
+	| "$"; s = STR; <e_var>
+let unary_expr :=
+	| primary_expr
+	| o = unop; e = unary_expr; { e_unop o e }
+let binary_expr :=
+	| unary_expr
+	| e1 = binary_expr; o = binop; e2 = unary_expr; { e_binop o e1 e2 }
